theories/LambdaCalculus/Lambda_undec.v
@@ -1,0 +1,42 @@
+(*
+  Author(s):
+    Andrej Dudenhefner (1)
+  Affiliation(s):
+    (1) TU Dortmund University, Dortmund, Germany
+*)
+
+(*
+  Undecidability Result(s):
+    Weak call-by-name leftmost outermost normalization for closed lambda-terms (wCBNclosed)
+    Strong normalization for closed lambda-terms (SNclosed)
+*)
+
+From Undecidability.Synthetic Require Import Undecidability ReducibilityFacts.
+
+Require Import Undecidability.LambdaCalculus.Lambda.
+From Undecidability.LambdaCalculus.Reductions Require
+  HaltLclosed_to_wCBNclosed
+  KrivineMclosed_HALT_to_SNclosed.
+Require Undecidability.L.Reductions.HaltL_to_HaltLclosed.
+
+Require Import Undecidability.L.L_undec.
+Require Import Undecidability.LambdaCalculus.Krivine_undec.
+
+(* Undecidability of weak call-by-name leftmost outermost normalization of closed terms *)
+Theorem wCBNclosed_undec : undecidable wCBNclosed.
+Proof.
+  apply (undecidability_from_reducibility HaltL_undec).
+  apply (reduces_transitive HaltL_to_HaltLclosed.reduction).
+  exact HaltLclosed_to_wCBNclosed.reduction.
+Qed.
+
+Check wCBNclosed_undec.
+
+(* Undecidability of strong normalization wrt. beta-reduction for closed lamda-terms *)
+Theorem SNclosed_undec : undecidable SNclosed.
+Proof.
+  apply (undecidability_from_reducibility KrivineMclosed_HALT_undec).
+  exact KrivineMclosed_HALT_to_SNclosed.reduction.
+Qed.
+
+Check SNclosed_undec.
